Completed add, find and remove function for blood bank

verification_finalised/bank/bank.dfy
@@ -3,7 +3,7 @@
 // on this sequence are all guarenteed to preserve the valid state of the 
 // system. These operations include: adding units, removing units, querying the
 // units, sorting the units.
-class BloodBank {
+class {:autocontracts} BloodBank {
 
     // Sequence of integers representing blood units
     var units: seq<int>;
@@ -22,17 +22,77 @@ class BloodBank {
     // an empty units sequence
     constructor () 
     modifies this;
+    ensures |units| == 0; 
     {
         units := [];
     }
 
-    // Add an new unit to the system
+    // Predicate to determine if the bank is full or not
+    predicate Full()
+    reads this;
+    {
+        |units| == 100000
+    }
 
-    // Remove unit from the system
+    // Add an new unit to the system
+    // This method ensures that an employee cannot add a unit if the storage is full,
+    // and that the same unit cannot be added to the bank twice.
+    method AddUnit(unit: int) 
+    requires !Full(); requires unit !in units;
+    ensures units == old(units) + [unit]
+    {
+        units := units + [unit];
+    }
+
+    // Finds the index of a given unit, if the unit does not exist 
+    // the function returns -1
+    method FindUnitIndex(unit: int) returns (key: int)
+    ensures units == old(units);
+    ensures key == -1 ==> unit !in units;
+    ensures key >=  0 ==> (key < |units| && units[key] == unit);    
+    ensures unit in units ==> (0<=key<|units| && units[key] == unit);
+    {
+        key := -1;
+        var index := 0; var limit := |units|;
+        
+        while index < limit 
+        decreases limit - index;
+        invariant index <= limit;
+        invariant key == -1 ==> unit !in units[..index];
+        invariant key >=  0 ==> (key < |units| && units[key] == unit);
+        {
+            if unit == units[index] { key := index; }
+            index := index + 1;
+        }
+    }
+
+    // Remove unit from the system, this function requires the unit 
+    // to be in the system since it does not make sense to remove a unit 
+    // which is not there.
+    method RemoveUnit(unit: int)
+    requires unit in units;
+    ensures |units| == |old(units)| - 1;
+    ensures forall i :: (0<=i<|old(units)| && old(units[i]) != unit) ==> old(units[i]) in units; 
+    {
+        var key := FindUnitIndex(unit);
+        units := units[..key] + units[(key+1)..];
+    }
 
     // Filter units from the system
 }
 
 // Sort list of blood units
+
+
+method Main() {
+    var bank := new BloodBank();
+
+    // Test 1: 
+    bank.AddUnit(1); assert 1 in bank.units;
+    bank.AddUnit(2); assert 2 in bank.units;
+    bank.RemoveUnit(1); assert 1 !in bank.units; assert 2 in bank.units;
+    var i2 := bank.FindUnitIndex(2); assert i2 == 0;
+}
+
 
     
